src/lang/Commit.v
@@ -1,0 +1,321 @@
+Require Import Omega.
+Require Import RelationClasses.
+
+Require Import sflib.
+Require Import paco.
+
+Require Import Axioms.
+Require Import Basic.
+Require Import DataStructure.
+Require Import Event.
+Require Import Time.
+Require Import Language.
+Require Import Memory.
+
+Set Implicit Arguments.
+
+
+Module Commit <: JoinableType.
+  Structure t_ := mk {
+    current: Snapshot.t;
+    released: LocFun.t Snapshot.t;
+    acquirable: Snapshot.t;
+  }.
+  Definition t := t_.
+
+  Definition init: t := mk Snapshot.init (LocFun.init Snapshot.init) Snapshot.init.
+
+  Inductive wf (commit:t) (mem:Memory.t): Prop :=
+  | wf_intro
+      (CURRENT: Memory.wf_snapshot commit.(current) mem)
+      (RELEASED: forall loc, Memory.wf_snapshot (commit.(released) loc) mem)
+      (ACQUIRABLE: Memory.wf_snapshot commit.(acquirable) mem)
+  .
+
+  Lemma future_wf
+        commit mem1 mem2
+        (WF: wf commit mem1)
+        (FUTURE: Memory.future mem1 mem2):
+    wf commit mem2.
+  Proof.
+    inv WF. econs; i; eapply Memory.future_wf_snapshot; eauto.
+  Qed.
+
+  Definition eq := @eq t.
+
+  Inductive le_ (lhs rhs:t): Prop :=
+  | le_intro
+      (CURRENT: Snapshot.le lhs.(current) rhs.(current))
+      (RELEASED: forall (loc:Loc.t), Snapshot.le (LocFun.find loc lhs.(released)) (LocFun.find loc rhs.(released)))
+      (ACQUIRABLE: Snapshot.le lhs.(acquirable) rhs.(acquirable))
+  .
+  Definition le := le_.
+
+  Global Program Instance le_PreOrder: PreOrder le.
+  Next Obligation.
+    ii. econs; reflexivity.
+  Qed.
+  Next Obligation.
+    ii. inv H. inv H0. econs; etransitivity; eauto.
+  Qed.
+
+  Definition join (lhs rhs:t): t :=
+    mk (Snapshot.join lhs.(current) rhs.(current))
+       (fun loc => Snapshot.join (lhs.(released) loc) (rhs.(released) loc))
+       (Snapshot.join lhs.(acquirable) rhs.(acquirable)).
+
+  Lemma join_comm lhs rhs: join lhs rhs = join rhs lhs.
+  Proof.
+    unfold join. f_equal.
+    - apply Snapshot.join_comm.
+    - extensionality loc. apply Snapshot.join_comm.
+    - apply Snapshot.join_comm.
+  Qed.
+
+  Lemma join_assoc a b c: join (join a b) c = join a (join b c).
+  Proof.
+    unfold join. s. f_equal.
+    - apply Snapshot.join_assoc.
+    - extensionality loc. apply Snapshot.join_assoc.
+    - apply Snapshot.join_assoc.
+  Qed.
+
+  Lemma join_l lhs rhs: le lhs (join lhs rhs).
+  Proof.
+    econs.
+    - apply Snapshot.join_l.
+    - i. apply Snapshot.join_l.
+    - apply Snapshot.join_l.
+  Qed.
+
+  Lemma join_r lhs rhs: le rhs (join lhs rhs).
+  Proof.
+    econs.
+    - apply Snapshot.join_r.
+    - i. apply Snapshot.join_r.
+    - apply Snapshot.join_r.
+  Qed.
+
+  Lemma join_spec lhs rhs o
+        (LHS: le lhs o)
+        (RHS: le rhs o):
+    le (join lhs rhs) o.
+  Proof.
+    inv LHS. inv RHS. econs.
+    - apply Snapshot.join_spec; eauto.
+    - i. apply Snapshot.join_spec; eauto.
+    - apply Snapshot.join_spec; eauto.
+  Qed.
+
+  Inductive read
+            (commit1:t) (loc:Loc.t) (ts:Time.t) (released:Snapshot.t) (ord:Ordering.t)
+            (commit2:t): Prop :=
+  | read_intro
+      (MONOTONE: le commit1 commit2)
+      (READABLE: Snapshot.readable commit1.(current) loc ts)
+      (READ: Time.le ts (Times.get loc commit2.(current).(Snapshot.reads)))
+      (ACQUIRE: forall (ORDERING: Ordering.le Ordering.acquire ord),
+          Snapshot.le released commit2.(current))
+      (ACQUIRABLE: Snapshot.le released commit2.(acquirable))
+  .
+
+  Inductive write
+            (commit1:t) (loc:Loc.t) (ts:Time.t) (released:Snapshot.t) (ord:Ordering.t)
+            (commit2:t): Prop :=
+  | write_intro
+      (MONOTONE: le commit1 commit2)
+      (WRITABLE: Snapshot.writable commit1.(current) loc ts)
+      (WRITE: Time.le ts (Times.get loc commit2.(current).(Snapshot.writes)))
+      (RELEASE: forall (ORDERING: Ordering.le Ordering.release ord),
+          Snapshot.le commit2.(current) (LocFun.find loc commit2.(Commit.released)))
+      (RELEASED: Snapshot.le (LocFun.find loc commit2.(Commit.released)) released)
+  .
+
+  Inductive fence
+            (commit1:t) (ord:Ordering.t)
+            (commit2:t): Prop :=
+  | fence_intro
+      (MONOTONE: le commit1 commit2)
+      (ACQUIRE: forall (ORDERING: Ordering.le Ordering.acquire ord),
+          Snapshot.le commit2.(acquirable) commit2.(current))
+      (RELEASE: forall (ORDERING: Ordering.le Ordering.release ord) loc,
+          Snapshot.le commit2.(current) (LocFun.find loc commit2.(released)))
+  .
+End Commit.
+
+Module CommitFacts.
+  Lemma wf_get
+        loc commit1 mem
+        (WF1: Commit.wf commit1 mem):
+    exists msg, Memory.get loc (Snapshot.writes (Commit.current commit1) loc) mem = Some msg.
+  Proof.
+    inversion WF1. inv CURRENT. inv WRITES.
+    specialize (WF loc). des. destruct msg. eauto.
+  Qed.
+
+  Lemma read_mon
+        commit1 commit2
+        (LE: Commit.le commit1 commit2):
+    Commit.read commit2 <5= Commit.read commit1.
+  Proof.
+    i. inv PR. econs; auto.
+    - etransitivity; eauto.
+    - eapply Snapshot.readable_mon; eauto.
+      apply LE.
+  Qed.
+
+  Lemma write_mon
+        commit1 commit2
+        (LE: Commit.le commit1 commit2):
+    Commit.write commit2 <5= Commit.write commit1.
+  Proof.
+    i. inv PR. econs; auto.
+    - etransitivity; eauto.
+    - eapply Snapshot.writable_mon; eauto.
+      apply LE.
+  Qed.
+
+  Lemma fence_mon
+        commit1 commit2
+        (LE: Commit.le commit1 commit2):
+    Commit.fence commit2 <2= Commit.fence commit1.
+  Proof.
+    i. inv PR. econs; auto. etransitivity; eauto.
+  Qed.
+
+  Definition read_min
+             loc ts released commit: Commit.t :=
+    (Commit.mk (Snapshot.mk
+                  (Times.incr loc ts (commit.(Commit.current).(Snapshot.reads)))
+                  commit.(Commit.current).(Snapshot.writes))
+               commit.(Commit.released)
+               (Snapshot.join released commit.(Commit.acquirable))).
+
+  Lemma read_min_spec
+        loc ts val released commit mem
+        (READABLE: Snapshot.readable (Commit.current commit) loc ts)
+        (MEMORY: Memory.wf mem)
+        (WF1: Commit.wf commit mem)
+        (WF2: Memory.get loc ts mem = Some (Message.mk val released)):
+    <<READ: Commit.read commit loc ts released Ordering.relaxed (read_min loc ts released commit)>> /\
+    <<WF: Commit.wf (read_min loc ts released commit) mem>> /\
+    <<CURRENT: forall loc' (LOC: loc' <> loc), Snapshot.le_on loc' (read_min loc ts released commit).(Commit.current) commit.(Commit.current)>>.
+  Proof.
+    splits.
+    - inv READABLE. econs; ss.
+      + econs; s; try reflexivity.
+        * econs; s; try reflexivity.
+          apply Times.incr_le.
+        * apply Snapshot.join_r.
+      + apply Times.incr_ts.
+      + apply Snapshot.join_l.
+    - econs; ss.
+      + econs; ss.
+        * eapply Memory.incr_wf_times; eauto. apply WF1.
+        * apply WF1.
+      + apply WF1.
+      + apply Memory.wf_snapshot_join.
+        * inv MEMORY. exploit WF; eauto.
+        * apply WF1.
+    - s. i. econs; s; [|reflexivity].
+      unfold Times.incr, LocFun.add, LocFun.find.
+      destruct (Loc.eq_dec loc' loc); [congruence|].
+      reflexivity.
+  Qed.
+
+  Lemma read_min_min
+        loc ts released commit1 commit2
+        (COMMIT2: Commit.read commit1 loc ts released Ordering.relaxed commit2):
+    Commit.le (read_min loc ts released commit1) commit2.
+  Proof.
+    inv COMMIT2. econs; s.
+    - econs; s.
+      + apply Times.incr_spec; auto. apply MONOTONE.
+      + apply MONOTONE.
+    - apply MONOTONE.
+    - apply Snapshot.join_spec; auto.
+      apply MONOTONE.
+  Qed.
+
+  Definition write_min
+             loc ts ord commit: Commit.t :=
+    (Commit.mk (Snapshot.mk
+                  commit.(Commit.current).(Snapshot.reads)
+                  (Times.incr loc ts commit.(Commit.current).(Snapshot.writes)))
+               (if Ordering.le Ordering.release ord
+                then LocFun.add
+                       loc (Snapshot.join
+                              (Snapshot.mk
+                                 commit.(Commit.current).(Snapshot.reads)
+                                 (Times.incr loc ts commit.(Commit.current).(Snapshot.writes)))
+                              (commit.(Commit.released) loc))
+                       commit.(Commit.released)
+                else commit.(Commit.released))
+               commit.(Commit.acquirable)).
+
+  Lemma write_min_spec
+        loc ts val released ord commit mem
+        (ORD: Ordering.le ord Ordering.release)
+        (WRITABLE: Snapshot.writable (Commit.current commit) loc ts)
+        (RELEASE: Snapshot.le ((write_min loc ts ord commit).(Commit.released) loc) released)
+        (MEMORY: Memory.wf mem)
+        (WF1: Commit.wf commit mem)
+        (WF2: Memory.get loc ts mem = Some (Message.mk val released))
+        (WF3: Memory.wf_snapshot released mem):
+    <<WRITE: Commit.write commit loc ts released ord (write_min loc ts ord commit)>> /\
+    <<WF: Commit.wf (write_min loc ts ord commit) mem>> /\
+    <<CURRENT: forall loc' (LOC: loc' <> loc), Snapshot.le_on loc' (write_min loc ts ord commit).(Commit.current) commit.(Commit.current)>>.
+  Proof.
+    splits.
+    - inv WRITABLE. econs; ss.
+      + econs; s; try reflexivity.
+        * econs; s; try reflexivity.
+          apply Times.incr_le.
+        * i. unfold LocFun.add, LocFun.find.
+          destruct ord; ss; try reflexivity.
+          destruct (Loc.eq_dec loc0 loc).
+          { subst. econs; s; apply Times.join_r. }
+          { reflexivity. }
+      + apply Times.incr_ts.
+      + destruct ord; ss. rewrite LocFun.add_spec.
+        destruct (Loc.eq_dec loc loc); [|congruence].
+        econs; s; apply Times.join_l.
+    - econs; ss.
+      + econs; ss.
+        * apply WF1.
+        * eapply Memory.incr_wf_times; eauto. apply WF1.
+      + destruct ord; ss; try apply WF1.
+        i. unfold LocFun.add, LocFun.find.
+        destruct (Loc.eq_dec loc0 loc); try apply WF1. subst.
+        apply Memory.wf_snapshot_join.
+        * econs; s; try apply WF1.
+          eapply Memory.incr_wf_times; try apply WF1. eauto.
+        * apply WF1.
+      + apply WF1.
+    - s. i. econs; s; [reflexivity|].
+      unfold Times.incr, LocFun.add, LocFun.find.
+      destruct (Loc.eq_dec loc' loc); [congruence|].
+      reflexivity.
+  Qed.
+
+  Lemma write_min_min
+        loc ts released ord commit1 commit2
+        (ORD: Ordering.le ord Ordering.release)
+        (COMMIT2: Commit.write commit1 loc ts released ord commit2):
+    Commit.le (write_min loc ts ord commit1) commit2.
+  Proof.
+    i. inv COMMIT2. econs; s.
+    - econs; s.
+      + apply MONOTONE.
+      + apply Times.incr_spec; auto. apply MONOTONE.
+    - destruct ord; ss; try apply MONOTONE.
+      i. unfold LocFun.add, LocFun.find.
+      destruct (Loc.eq_dec loc0 loc); try apply MONOTONE. subst.
+      apply Snapshot.join_spec.
+      + etransitivity; [|apply RELEASE]; auto. econs; s.
+        { apply MONOTONE. }
+        { apply Times.incr_spec; auto. apply MONOTONE. }
+      + apply MONOTONE.
+    - apply MONOTONE.
+  Qed.
+End CommitFacts.
